MultiScalarMul_Abstract_Soundness.ec
@@ -11,48 +11,23 @@ require import IterationProps.
 section.
 
 declare module O <: OutCalls.
- 
-declare axiom tablePT_ph parg varg : phoare [ O.getPT : arg = (parg,varg)
-   ==> res.`1 => (res.`2 = (fun (j i : int) =>  (i *** (parg j)) +++ - varg)  /\ (forall i j, res.`2 i j <> idR) )   ] = 1%r.
 
+declare axiom O_lossless : islossless O.getU. 
 
-lemma tablePT parg varg : hoare [ O.getPT : arg = (parg,varg)
-   ==> res.`1 => (res.`2 = (fun (j i : int) =>  (i *** (parg j)) +++ - varg)  /\ (forall i j, res.`2 i j <> idR) )   ].
-proof. conseq (tablePT_ph parg varg). auto. qed.
-   
-
-(* lemma helpereqs argacc argtable argic args  :  *)
-(*  equiv [ SimpleComp.completeAddLoop ~ SimpleComp.incompleteAddLoop :  *)
-(*   arg{2} = (argacc, argtable, argic, args) /\ ={acc,table,ic,s} *)
-(*        /\ (forall i j, table{1} i j <> idR) *)
-(*      ==>  res{2}.`1 => (res{1} = res{2}.`2)]. *)
-(* proc. *)
-(* while (={jc,acc,table,aux,s,ic} /\ (flag{2} => ={vahe}) *)
-(*  /\ (forall i j, table{1} i j <> idR)). *)
-(*  wp. skip. progress. *)
-(*    have -> : vahe{1} = vahe{2}. smt(). *)
-(* rewrite same_res.  admit. *)
-(*   smt(). *)
-(*   smt().  *)
-(*   smt(). *)
-(*   (* smt(). *) *)
-(* wp. skip. progress.  *)
-(* qed. *)
-
-
-lemma multieqs argP args argU  :
+lemma multieqs2 argP args argU  :
  equiv [ SimpleComp.multiScalarMulMain_Perfect 
-        ~ MultiScalarMul(O).multiScalarMulI :
+        ~ SimpleComp.multiScalarMulMain_Opt_Corrected :
   arg{2} = (argP, args, argU) /\ ={P,s,U} /\ ={glob O}
      ==>  res{2}.`1 => (res{1} = res{2}.`2)].
 proc.
 wp.
-while ((flag{2} => ={table,acc,U,s} /\ (forall i j, table{2} i j <> idR)) /\ (flag{2} => flagaux{2}) /\ ={ic}  ).
+inline SimpleComp.multiScalarMulMain_Opt. wp.
+while ((flag0{2} => ={table,acc,U,s} /\ (forall i j, table{2} i j <> idR)) /\ (flag0{2} => flagaux{2}) /\ ={ic} /\ s{1} = s0{2}  ).
 wp.
 inline SimpleComp.completeAddLoop.
 inline SimpleComp.incompleteAddLoop.   
 wp.
-while ((flag{2} /\ flag0{2} => ={vahe, acc0,table0,aux0,s0,ic0} /\ (forall i j, table0{2} i j <> idR) /\ vahe{2} <> idR) /\ ={jc0} ).
+while ((flag0{2} /\ flag1{2} => ={vahe, acc0,table0,aux0,s0,ic0} /\ (forall i j, table0{2} i j <> idR) /\ vahe{2} <> idR) /\ ={jc0} /\ s0{1} = s1{2} ).
  wp. skip. progress.
    have -> : vahe{1} = vahe{2}. smt().
 rewrite same_res. 
@@ -73,19 +48,19 @@ ecall {1} (doublewtimes_spec_ph acc{1} w).
 ecall {2} (doublewtimes_spec_ph acc{2} w).
 skip. progress. 
 smt(w_pos). smt(). smt(). smt().
-smt(). smt().
+smt(). 
 apply no_order_two_elems. smt(w_pos).
 smt(). smt(). smt().
 smt(). smt().    
 wp. 
-ecall {2} (tablePT_ph P{2} v{2}).    
-wp. skip. progress. smt(). smt().
-have -> :     acc_L = acc_R. smt(). auto.
+ skip. progress. admit. smt().
 qed.
 
 
+
+
 lemma multiscalarI_spec_ph argP args  argU : 
- phoare [ MultiScalarMul(O).multiScalarMulI : 
+ phoare [ SimpleComp.multiScalarMulMain_Opt_Corrected : 
   arg = (argP, args, argU) 
      ==>  res.`1 => res.`2 = (multiScalarMulR  args argP)  ] = 1%r.
 proof.
@@ -95,13 +70,13 @@ have ih: 1%r = Pr[SimpleComp.multiScalarMulMain_Perfect(P{m}, s{m}, U{m}) @ &m
   : res = multiScalarMulR args argP].
 byphoare (_: arg = (argP, args, argU) ==> _).
 conseq (multiscalarR_spec_ph argP args argU). smt(). auto.
-have : Pr[MultiScalarMul(O).multiScalarMulI(P{m}, s{m}, U{m}) @ &m :
+have : Pr[SimpleComp.multiScalarMulMain_Opt_Corrected(P{m}, s{m}, U{m}) @ &m :
    res.`1 => res.`2 = multiScalarMulR args argP] >=
 Pr[SimpleComp.multiScalarMulMain_Perfect(P{m}, s{m}, U{m}) @ &m :
    res = multiScalarMulR args argP].
 byequiv (_: ={glob O} /\ arg{2} = (P{m}, s{m}, U{m}) /\ arg{1} = (P{m}, s{m}, U{m}) ==> res{2}.`1 => res{2}.`2 = res{1} ).
 proc*.
-ecall (multieqs argP args argU).
+ecall (multieqs2 argP args argU).
 skip. progress. smt(). smt(). smt(). 
 auto.
 smt().
@@ -111,27 +86,22 @@ smt.
 qed.
 
 
-lemma multiscalarI_spec_h argP args  argU : 
- hoare [ MultiScalarMul(O).multiScalarMulI : 
-  arg = (argP, args, argU) 
-     ==>  res.`1 => res.`2 = (multiScalarMulR  args argP)  ] .
-conseq (multiscalarI_spec_ph argP args argU).
-qed.   
-
-
 lemma multiscalar_spec_h argP args : 
- hoare [ MultiScalarMul(O).multiScalarMul : 
+ phoare [ MultiScalarMul(O).multiScalarMul : 
   arg = (argP, args) 
-     ==>  res.`1 => res.`2 = (multiScalarMulR  args argP)  ] .
+     ==>  res.`1 => res.`2 = (multiScalarMulR  args argP)  ] = 1%r .
 proc.
 seq 1 : #pre.
 call (_: true). auto.
-sp. if.
-  ecall (multiscalarI_spec_h P s (embed u_cand)).
-   skip. progress.
-wp. skip.
-smt().
-qed.   
+call (_: true). auto.
+apply O_lossless.
+ auto.   
+
+exists* u_cand. elim*. move => u_candV.
+call (multiscalarI_spec_ph  argP args (embed u_candV)).
+wp.   skip. progress.
+hoare. simplify. call(_:true). auto. auto.
+ qed.   
 
 
 end section.
